otp/OTP_verif.v
@@ -2,7 +2,6 @@ Require Import List.
 Import ListNotations.
 Require Import String.
 
-(* Borrow from CompCert *)
 Require Import Cryptol.Coqlib.
 Require Import Cryptol.Bitvectors.
 
@@ -67,22 +66,28 @@ Qed.
 
 Lemma bool_destr : forall (b: bool),
     (if b then true else false) = b. 
-  Proof. 
-    destruct b; auto. 
-  Qed.
+Proof. 
+  destruct b; auto. 
+Qed.
 
-  
-Lemma otp_equiv' : forall key msg,
-  has_type key byte -> 
-  has_type msg byte ->
-  exists l,  
+
+Theorem otp_equiv :
+  forall key msg,
+    (* key is the right type *)
+    has_type key byte ->
+    (* msg is the right type *)
+    has_type msg byte ->
+    (* applying the encrypt function to the key and value gives the model *)
     eager_eval_expr ge tempty sempty
-                    (EApp (EApp (EVar encrypt) (EValue key)) (EValue msg)) (to_sval l)
-    /\ otp_encrypt key msg = l.
+                    (EApp (EApp (EVar encrypt) (EValue key)) (EValue msg))
+                    (to_sval (otp_encrypt key msg)).
 Proof.
-  intros. inversion H. do 9 (destruct l; simpl in H1; try omega).
-
+  intros.
+  (* break apart bytes into elements *)
+  inversion H. do 9 (destruct l; simpl in H1; try omega).
+  inversion H0. do 9 (destruct l; simpl in H5; try omega).
   subst.
+  (* each element is a bit *)
   repeat match goal with
          | [ H : Forall _ _ |- _ ] => inversion H; clear H
          end;
@@ -90,71 +95,13 @@ Proof.
            | [ H : has_type _ tbit |- _ ] => inversion H; clear H
            end;
     subst.
-  inversion H0. clear H0. inversion H4. clear H4.
-  symmetry in H0. rewrite <- length_zero_iff_nil in H0. omega.
-  inversion H6. symmetry in H8. rewrite <- length_zero_iff_nil in H8.
-  rewrite length_cons in H8. rewrite H7 in H8. omega.
-  inversion H9. symmetry in H11. rewrite <- length_zero_iff_nil in H11.
-  rewrite length_cons in H11. rewrite H10 in H11. subst.
-  rewrite <- length_cons in H2. omega.
-  subst.
 
-  inversion H12. symmetry in H3. rewrite <- length_zero_iff_nil in H3.
-  do 3 (rewrite <- length_cons in H2). omega. subst.
-  
-  inversion H5. symmetry in H7. rewrite <- length_zero_iff_nil in H7.
-  do 4 (rewrite <- length_cons in H2). omega. subst. 
-  
-  inversion H10. symmetry in H13. rewrite <- length_zero_iff_nil in H13. 
-  do 5 (rewrite <- length_cons in H2). omega. subst.
-  
-  inversion H14. symmetry in H15. rewrite <- length_zero_iff_nil in H15. 
-  do 6 (rewrite <- length_cons in H2). omega. subst.
- 
-  inversion H16. symmetry in H17. rewrite <- length_zero_iff_nil in H17. 
-  do 7 (rewrite <- length_cons in H2). omega. subst.
-
-  inversion H18. subst. Focus 2. subst. simpl in H2. omega. 
-
-  repeat match goal with
-    | [H : has_type _ tbit |- _] => inversion H; clear H end. 
-
-  eexists. 
-  split. 
-
+  (* evaluate the function *)
   e. e. g. e. e. e. e. e. e. e.
   g.
   e. e. lv. e. lv. e.
   lv. lv.
-  simpl. f_equal.
-  unfold to_sval. 
-  instantiate (1:= eseq
-                     (
-                       (ebit (if b6 then if b14 then false else true else b14)) ::
-                                                                                (ebit (if b5 then if b13 then false else true else b13)) ::
-                                                                                (ebit (if b4 then if b12 then false else true else b12)) ::
-                                                                                (ebit (if b3 then if b11 then false else true else b11)) ::
-                                                                                (ebit (if b2 then if b10 then false else true else b10)) ::
-                                                                                (ebit (if b1 then if b9 then false else true else b9)) ::
-                                                                                (ebit (if b0 then if b8 then false else true else b8)) ::
-                                                                                (ebit (if b then if b7 then false else true else b7)) :: nil )). 
-  simpl. 
-  reflexivity. 
-  simpl. 
-  unfold xorb.    
-  repeat rewrite bool_destr. 
-  reflexivity. 
+  simpl. unfold xorb.
+  repeat rewrite bool_destr.
+  reflexivity.
 Qed.
-
-Theorem otp_equiv : forall key msg,
-  has_type key byte -> 
-  has_type msg byte ->
-  eager_eval_expr ge tempty sempty
-                  (EApp (EApp (EVar encrypt) (EValue key)) (EValue msg)) (to_sval (otp_encrypt key msg)).
-Proof.
-  intros.
-  edestruct otp_equiv'. exact H. exact H0.
-  destruct H1.
-  subst x.
-  assumption.
-Qed.  
